state/Compiler.fst
@@ -155,7 +155,7 @@ type ctx_tgt2 (i:tgt_interface2) =
   write : ttl_write fl inv prref hrel ->
   alloc : ttl_alloc fl inv prref hrel  ->
   p:i.pt fl inv prref hrel ->
-  ST int fl (fun h0 -> inv h0) (fun h0 _ h1 -> h0 `hrel` h1 /\ inv h1) (** TODO: to check if the program should be an arrow because we don't enforce prref **)
+  STFlag int fl (fun h0 -> inv h0) (fun h0 _ h1 -> h0 `hrel` h1 /\ inv h1) (** TODO: to check if the program should be an arrow because we don't enforce prref **)
 
 type prog_tgt2 (i:tgt_interface2) =
   i.pt AllOps (Mktuple3?._1 default_spec) (Mktuple3?._2 default_spec) (Mktuple3?._3 default_spec)
